thys/AVL-Trees/AVL.thy
@@ -1,5 +1,5 @@
 (*  Title:      AVL Trees
-    ID:         $Id: AVL.thy,v 1.9 2006-05-26 19:45:29 nipkow Exp $
+    ID:         $Id: AVL.thy,v 1.10 2007-07-22 20:44:18 makarius Exp $
     Author:     Tobias Nipkow and Cornelia Pusch,
                 converted to Isar by Gerwin Klein
                 contributions by Achim Brucker, Burkhart Wolff and Jan Smaus
@@ -69,9 +69,9 @@ primrec
 "ht ET = 0"
 "ht (MKT x l r h) = h"
 
-constdefs
- mkt :: "'a \<Rightarrow> 'a tree \<Rightarrow> 'a tree \<Rightarrow> 'a tree"
-"mkt x l r \<equiv> MKT x l r (max (ht l) (ht r) + 1)"
+definition
+ mkt :: "'a \<Rightarrow> 'a tree \<Rightarrow> 'a tree \<Rightarrow> 'a tree" where
+"mkt x l r = MKT x l r (max (ht l) (ht r) + 1)"
 
 consts
  l_bal :: "'a * 'a tree * 'a tree \<Rightarrow> 'a tree"
