thys/MiniML/Maybe.thy
@@ -1,5 +1,5 @@
 (* Title:     HOL/MiniML/Maybe.thy
-   ID:        $Id: Maybe.thy,v 1.6 2004-08-18 07:24:54 nipkow Exp $
+   ID:        $Id: Maybe.thy,v 1.7 2007-07-22 20:44:19 makarius Exp $
    Author:    Wolfgang Naraschewski and Tobias Nipkow
    Copyright  1996 TU Muenchen
 *)
@@ -10,12 +10,12 @@ theory Maybe
 imports Main
 begin
 
-constdefs
-  option_bind :: "['a option, 'a => 'b option] => 'b option"
-  "option_bind m f == case m of None => None | Some r => f r"
+definition
+  option_bind :: "['a option, 'a => 'b option] => 'b option" where
+  "option_bind m f = (case m of None => None | Some r => f r)"
 
 syntax "@option_bind" :: "[pttrns,'a option,'b] => 'c" ("(_ := _;//_)" 0)
-translations "P := E; F" == "option_bind E (%P. F)"
+translations "P := E; F" == "CONST option_bind E (%P. F)"
 
 
 -- "constructor laws for @{text option_bind}"
